Veritas.Verifier.EAC.fst
@@ -1,11 +1,13 @@
 module Veritas.Verifier.EAC
 
 open FStar.Seq
+open Veritas.BinTree
 open Veritas.EAC
 open Veritas.Hash
 open Veritas.Interleave
 open Veritas.Key
 open Veritas.MultiSetHash
+open Veritas.Record
 open Veritas.SeqAux
 open Veritas.SeqMachine
 open Veritas.State
@@ -13,72 +15,91 @@ open Veritas.Verifier
 open Veritas.Verifier.CorrectDefs
 
 type its_log (n:nat) = 
-  s:seq (idx_elem #vlog_entry n){g_verifiable (partition_idx_seq s) /\
-                                 g_hash_verifiable (partition_idx_seq s)}
+  s:seq (idx_elem #vlog_entry n){g_verifiable (partition_idx_seq s)}
+
+(* extended time sequence log (with evict values) *)
+let time_seq_ext (#n:nat) (itsl: its_log n): (le:vlog_ext{project_seq itsl = to_vlog le}) =
+  admit()
+
+(* the prefix of an its log *)
+let its_prefix (#n:nat) (itsl: its_log n) (i:nat{i <= length itsl}): 
+  (itsl':its_log n{length itsl' = i}) =
+  let itsl': seq (idx_elem #vlog_entry n) = prefix itsl i in
+  let gl = partition_idx_seq itsl in
+  let idgl = g_tid_vlog gl in
+  
+  let gl' = partition_idx_seq itsl' in
+  let idgl' = g_tid_vlog gl' in
+
+  let aux (id:nat{id < n}):
+    Lemma (requires True)
+          (ensures (t_verifiable (index idgl' id)))
+          [SMTPat (t_verifiable (index idgl' id))]    
+    = 
+    let (_,l') = index idgl' id in
+    //let (_,l) = index idgl id in    
+    lemma_partition_idx_prefix_comm itsl i  id;
+    lemma_verifiable_implies_prefix_verifiable (index idgl id) (length l');
+    ()
+  in
+  itsl'
+
+let lemma_its_prefix_ext (#n:nat) (itsl:its_log n) (i:nat{i <= length itsl}):
+  Lemma (time_seq_ext (its_prefix itsl i) = prefix (time_seq_ext itsl) i) = 
+  admit()
+
+(* the eac state of a key after processing an eac_log *)
+let eac_state_key (le: vlog_ext) (k:key): eac_state = 
+  let lek = partn eac_sm k le in
+  seq_machine_run eac_smk lek
+
+(* the state of a verifier thread after processing entries in a log *)
+let verifier_thread_state (#n:nat) (itsl: its_log n) (id:nat{id < n}): (st:vtls{Valid? st}) = 
+  let gl = partition_idx_seq itsl in
+  assert(t_verifiable (index (attach_index gl) id));
+  t_verify id (index gl id)
 
 (* generalized single- and multi-set hash collision *)
 type hash_collision_gen =
   | SingleHashCollision: hc: hash_collision -> hash_collision_gen
   | MultiHashCollision: hc: ms_hash_collision -> hash_collision_gen
 
-(* extended time sequence log (with evict values) *)
-let time_seq_ext (#n:nat) (itsl: its_log n): (le:vlog_ext{project_seq itsl = to_vlog le}) =
-  admit()
+(* construct a hash collision from a contradiction *)
+let hash_collision_contra (_:unit{False}): hash_collision_gen = 
+  SingleHashCollision (Collision (DVal Null) (DVal Null))
+
+(* 
+ * when the eac state of a key is Init (no operations on the key yet) no 
+ * thread contains the key in its store 
+ *)
+let lemma_eac_state_init_store (#n:nat) (itsl: its_log n) (k: key{k <> Root}) (id:nat{id < n}):
+   Lemma (not (store_contains (thread_store (verifier_thread_state itsl id)) k)) 
+   = admit()
 
 type eac_ts_log (#n:nat) = itsl: its_log n {is_eac_log (time_seq_ext itsl)}
 type non_eac_ts_log (#n:nat) = itsl: its_log n {not (is_eac_log (time_seq_ext itsl))}
 
+(* the entry that causes the eac_invalidation *)
+let invalidating_log_entry (#n:nat) (itsl: non_eac_ts_log #n): vlog_entry_ext = 
+  let tsle = time_seq_ext itsl in  
+  let i = max_eac_prefix tsle in  
+  index tsle i
+
+(* the key that causes the eac_invalidation *)
 let eac_invalidating_key (#n:nat) (itsl: non_eac_ts_log #n): key =
-  let tsle = time_seq_ext itsl in
+  vlog_entry_key (invalidating_log_entry itsl)
 
-  (* maximum eac valid prefix *)
-  let i = max_eac_prefix tsle in
-
-  (* ee is the entry causing eac invalidation *)
-  let ee = index tsle i in
-  
-  (* the key causing the invalidation *)
-  partn_fn eac_sm ee
-
-
+(* last valid eac state *)
 let last_valid_eac_state (#n:nat) (itsl: non_eac_ts_log #n): eac_state = 
-
-  let tsle = time_seq_ext itsl in
-  
+  let tsle = time_seq_ext itsl in  
   let i = max_eac_prefix tsle in
-
-  (* maximum eac prefix *)
-  let tslei = prefix tsle i in
-
-  (* minimum non-eac prefix *)
-  let tslei' = prefix tsle (i + 1) in
-
-  lemma_first_invalid_key eac_sm tsle;
-
-  (* ee is the entry causing eac invalidation *)
-  let ee = index tsle i in
-  
-  (* the key causing the invalidation *)
   let k = eac_invalidating_key itsl in
-
-  (* log entries of only key k *)
-  let tslek = partn eac_sm k tsle in
-
-  (* j the index in tslek causing invalidation *)
-  let j = max_valid_prefix eac_smk tslek in
-  //assert(filter_index_inv_map (iskey vlog_entry_key k) tsle i = j);  
-  //assert(vlog_entry_key ee = k);
-  //assert(index tslek j = ee);
-
-  let tslekj = prefix tslek j in
-  assert(valid eac_smk tslekj);
+  eac_state_key (prefix tsle i) k
   
-  let st = seq_machine_run eac_smk tslekj in
-  assert(st <> EACFail);
-
-  st
-
-let lemma_non_eac_time_seq_implies_hash_collision (#n:nat) (itsl: non_eac_ts_log #n): hash_collision_gen = 
+(* applying the invalidating entry on the last valid state produces EAC failure *)
+let lemma_invalidation (#n:nat) (itsl: non_eac_ts_log #n):
+  Lemma (EACFail <> last_valid_eac_state itsl /\
+         EACFail = eac_add (invalidating_log_entry itsl) (last_valid_eac_state itsl)) =            
   let tsl = project_seq itsl in
   let tsle = time_seq_ext itsl in
   
@@ -94,7 +115,8 @@ let lemma_non_eac_time_seq_implies_hash_collision (#n:nat) (itsl: non_eac_ts_log
 
   (* ee is the entry causing eac invalidation *)
   let ee = index tsle i in
-  
+  assert(ee = invalidating_log_entry itsl);
+
   (* the key causing the invalidation *)
   let k = eac_invalidating_key itsl in
 
@@ -108,17 +130,70 @@ let lemma_non_eac_time_seq_implies_hash_collision (#n:nat) (itsl: non_eac_ts_log
   //assert(index tslek j = ee);
 
   let tslekj = prefix tslek j in
-  assert(valid eac_smk tslekj);
-  
+  assert(valid eac_smk tslekj);  
+
   let st = seq_machine_run eac_smk tslekj in
   assert(st <> EACFail);
+
+  // filtering out k-entries in tslei is the as taking the prefix j in tslekj
+  lemma_filter_prefix_comm (iskey vlog_entry_key k) tsle i;
   assert(st = last_valid_eac_state itsl);
-  
+
   lemma_reduce_prefix EACInit eac_add (prefix tslek (j + 1)) j;  
   lemma_reduce_singleton st eac_add (suffix (prefix tslek (j + 1)) 1);
   assert(eac_add ee st = EACFail);
-  
+
+  ()         
+
+(* eac invalidation is caused by a get as the first operation *)
+let lemma_non_eac_init_get (#n:nat) 
+  (itsl: non_eac_ts_log #n{last_valid_eac_state itsl = EACInit /\
+                           Get? (to_vlog_entry (invalidating_log_entry itsl))}): hash_collision_gen = 
+  let tsle = time_seq_ext itsl in  
+  let i = max_eac_prefix tsle in
+  let ee = invalidating_log_entry itsl in
+  let e = to_vlog_entry ee in
+  let k = vlog_entry_key ee in
+  let st = last_valid_eac_state itsl in
+  assert(st = EACInit);
+  assert(is_data_key k);
+  assert(length tsle = length itsl);
+  let itsli = its_prefix itsl i in
+  let tslei = time_seq_ext itsli in
+  lemma_its_prefix_ext itsl i;
+  assert(tslei = prefix tsle i);
+
+  assert(eac_state_key tslei k = st);
+  let (_,id) = index itsl i in
+  assert(id < n);  
+  lemma_eac_state_init_store itsli k id;
+
+  let gli = partition_idx_seq itsli in
+  let igli = attach_index gli in
+  let tsli_id = verifier_thread_state itsli id in
+  assert(not (store_contains (thread_store tsli_id) k));
+
+  let itsli' = its_prefix itsl (i + 1) in
+  let gli' = partition_idx_seq itsli' in
+  let tsli'_id = verifier_thread_state itsli' id in 
+  assert(Valid? tsli'_id);
+
+  lemma_partition_idx_extend1 itsli';
+  assert(index gli' id = append1 (index gli id) (fst (telem itsli')));
+  assert(telem itsli' = index itsl i);
+  let ec = fst (index itsl i) in
+  let tslei' = time_seq_ext itsli' in
+
+  admit()
+
+let lemma_non_eac_time_seq_implies_hash_collision (#n:nat) (itsl: non_eac_ts_log #n): hash_collision_gen = 
+  let st = last_valid_eac_state itsl in
+  let ee = invalidating_log_entry itsl in
   match st with
-  | EACInit -> admit()
+  | EACInit -> (
+      match ee with 
+      | NEvict (Get _ _) -> lemma_non_eac_init_get itsl            
+      | _ -> admit()
+    )
   | EACInCache m v -> admit()
   | EACEvicted m v -> admit()
